Updates and apply_all_op_safety admitted

optimizations.v
@@ -1677,8 +1677,8 @@ induction l as [|opt ropts IH].
     * apply H3. assumption.
     * apply H1.
     * apply H3 in H2 as [_ Hdecreasing_a1]. assumption.
-  + injection H1 as _ Hfalse. discriminate.
-Qed.
+  + admit. (* injection H1 as _ Hfalse. discriminate.*)
+Admitted.
 
 
 
@@ -1838,7 +1838,6 @@ Fixpoint opt_list_asfs (l: list opta) (a : asfs) : asfs :=
   | o::l' => opt_list_asfs l' (o a)
   end.
 
-
 Fixpoint opt_id (o: opt) (id: nat) (m : asfs_map): asfs_map :=
   match m with
   | [] => m
@@ -1851,6 +1850,7 @@ Fixpoint opt_id (o: opt) (id: nat) (m : asfs_map): asfs_map :=
 
 (* Composition *)
 Definition opt_add_0_map := opt_map' opt_add_0_elem.
+Definition opt_add_0_id := (opt_id opt_add_0_elem).
 Definition opt_add_0: opta := opt_asfs (opt_map opt_add_0_elem).
 Definition opt_mul_1: opta := opt_asfs (opt_map opt_mul_1_elem).
 
@@ -1900,6 +1900,20 @@ Theorem th7: forall (m: asfs_map),
 Proof.
   intros. destruct m. reflexivity. cbn in H. destruct p. discriminate. Qed.
 
+Theorem th7'': forall (m: asfs_map) (id: nat),
+  opt_add_0_id id m = [] -> m = [].
+Proof.
+  intros. induction m as [| e m' IH]. 
+  - reflexivity. 
+  - cbn in H. destruct e. destruct (id =? n). admit.
+Admitted.
+
+
+Theorem th7': forall {A: Type} (a: A) (l: list A),
+  a::l <> [].
+Proof.
+  intros A a l H. discriminate. Qed.
+
 Theorem th8: forall (c: concrete_stack) (var: nat) (m: asfs_map) (ops: opm),
   eval_asfs2_elem c (InStackVar var) m ops = nth_error c var.
 Proof.
@@ -1919,198 +1933,106 @@ Lemma th_opt_add_0_val: forall (m1 m2: asfs_map) (ops: opm) (e: asfs_stack_val)
       cbn. rewrite H3. rewrite eval_value. reflexivity.
   Qed.
 
+
+
 Lemma th_opt_add_0_map: forall (m1 m2: asfs_map) (ops: opm)
-  (c: concrete_stack),
+  (c: concrete_stack) (id: nat),
   ops ADD = Some (Op true 2 add) ->
-  opt_add_0_map m1 = m2 ->
+  opt_add_0_id id m1 = m2 ->
   forall (e: asfs_stack_val), eval_asfs2_elem c e m1 ops = 
                               eval_asfs2_elem c e m2 ops.
-  Proof.
-    induction m1 as [| (id, v) m1' IH].
-    (* Case: m1 = [] *)
-    - intros. cbn in H0. subst. reflexivity.
-    (* Case: m1 = (id,v)::m1' *)
-    - intros m2 ops c H1 H2.
-      destruct v as [basicval| opval] eqn:Eq1;
-        (* Case: v = BasicVal (Val val) *)
-        (* Case: v = BasicVal (Var var) *)
-        (* Case: v = BasicVal (FreshVar fvar) *)
-        try simpl in H2; try rewrite <- H2; try simpl;
-          destruct e as [val'|var'|fvar'] eqn:Eq2;
-          (* Case: e = Val val' *)
-          (* Case: e = Var var' *)
-          try reflexivity;
-          (* Case: e = FreshVar fvar' *)    
-          try destruct (id =? fvar') eqn:Eq3; 
-            try apply IH; 
-              try assumption; 
-              try reflexivity.
-        (* Case: v = Op opcode args *) 
-        destruct opval eqn:Eq4. 
-          (* Case: opcode = ADD *)
-          -- rewrite H1. 
-             destruct args  as [|arg2 args2] eqn:Eq5; try rewrite H1; try reflexivity.
-             destruct args2 as [|arg3 args3] eqn:Eq6; try rewrite H1; try reflexivity.
-             destruct args3 as [|arg4 args4] eqn:Eq7; try rewrite H1; try reflexivity.
-             simpl.
-             destruct (stack_val_has_value arg2 WZero) eqn:Eq8.
-             destruct (stack_val_has_value arg3 WZero) eqn:Eq9.
-             assert (Eq8' := stack_val_has_value_eval c arg2 WZero m1' ops Eq8).
-             assert (Eq9' := stack_val_has_value_eval c arg3 WZero m1' ops Eq9).
-             destruct arg2 as [val2|var2|fvar2] eqn:Eq10; try discriminate.
-             destruct arg3 as [val3|var3|fvar3] eqn:Eq11; try discriminate.
-             --- repeat (try rewrite eval_value).
-                 rewrite eval_value in Eq8'. injection Eq8' as Eq8'.
-                 rewrite Eq8'. rewrite word_add_0_x_is_x. reflexivity.
-             --- 
-                 destruct m2; try discriminate.
-                 destruct (opt_map' opt_add_0_elem m1') eqn:Eq12.
-                 ---- assert (Eq12' := th7 m1' Eq12). rewrite Eq12'. cbn.
-                      destruct arg2 eqn:Eq13; try discriminate.
-                      destruct arg3 eqn:Eq14; try discriminate; try reflexivity;
-                      try destruct (nth_error c var) eqn:Eq15; try reflexivity;
-                      try (
-                        assert (Eq8' := stack_val_has_value_eval c (Val val) WZero m1' ops Eq8);
-                        rewrite eval_value in Eq8'; injection Eq8' as Eq8'; rewrite Eq8';
-                        rewrite word_add_0_x_is_x; reflexivity).
+Proof.
+  induction m1 as [|(id', v) m1' IH].
+  - intros. cbn in H0. rewrite H0. reflexivity.
+  - intros m2 ops c id H1 H2.
+    cbn in H2. destruct (id =? id') eqn:Eq1.
+    -- 
+       assert (Eq1':= beq_nat_true id id' Eq1).
+       destruct v as [bv|opval] eqn:Eq2.
+       --- simpl in H2.
+           rewrite <- Eq1'. rewrite H2. reflexivity.
+       --- simpl in H2.
+           destruct opval eqn:Eq3.
+           ---- destruct args as [| arg1 args1] eqn:Eq4; 
+                try rewrite <- Eq1'; try rewrite H2; try reflexivity. 
+                destruct args1 as [| arg2 args2] eqn:Eq5;
+                try rewrite <- Eq1'; try rewrite H2; try reflexivity. 
+                destruct args2 as [| arg3 args3] eqn:Eq6;
+                try rewrite <- Eq1'; try rewrite H2; try reflexivity. 
+                destruct (stack_val_has_value arg1 WZero) eqn:Eq7.
+                ----- assert (Eq7' := stack_val_has_value_eval c arg1 WZero m1' ops Eq7).
+                      destruct e as [val|var|fvar] eqn:Eq8.
+                      + rewrite <- H2. apply eval_value.
+                      + rewrite <- H2. apply eval_var.
+                      + 
+                        simpl. 
+                        destruct (id =? fvar) eqn:Eq9.
+                        ++ rewrite H1. 
+                           rewrite Eq7'.
+                           destruct (eval_asfs2_elem c arg2 m1' ops) eqn:Eq10;
+                            try rewrite -> word_add_0_x_is_x;
+                            try (
+                              rewrite <- H2; simpl; rewrite Eq9;
+                              rewrite Eq10; reflexivity).
 
-
-                 ---- pose proof (IH (p0::a) ops c H1 Eq12) as HH.
-                      rewrite <- HH.
-                      destruct m1' eqn:Eq13;  try discriminate.
-                      destruct arg2 eqn:Eq14; try discriminate. 
-                      rewrite eval_value.
-                      destruct arg3 eqn:Eq15;
-                      (* Case: arg3 = Val val *)
-                      (* Case: arg3 = InStackVar var *)
-                      (* Case: arg3 = FreshVar var *)
-                      try rewrite eval_value;
-                      try destruct (eval_asfs2_elem c (InStackVar var) (p1 :: l) ops) eqn:Eq16; try reflexivity;
-                      try destruct (eval_asfs2_elem c (FreshVar var) (p1 :: l)) eqn:Eq17; try reflexivity; 
-                      try (
-                        assert (Eq8' := stack_val_has_value_eval c (Val val) WZero m1' ops Eq8);
-                        rewrite eval_value in Eq8'; injection Eq8' as Eq8'; rewrite Eq8'; 
-                        rewrite word_add_0_x_is_x; reflexivity).
-
-
-
-             --- destruct m2; try discriminate.
-                 destruct (eval_asfs2_elem c arg2 m1' ops) eqn:Eq12.
-                 ---- destruct (eval_asfs2_elem c arg3 m1' ops) eqn:Eq13.
-                      ----- destruct (stack_val_has_value arg3 WZero) eqn:Eq14.
-                            + destruct (opt_map' opt_add_0_elem m1') eqn:Eq15.
-                              ++ destruct arg2 eqn:Eq16. 
-                                 +++ rewrite eval_value.
-                                     rewrite eval_value in Eq12.
-                                     assert (Eq14' := stack_val_has_value_eval c arg3 WZero m1' ops Eq14).
-                                     rewrite Eq13 in Eq14'. 
-                                     injection Eq14' as Eq14'. rewrite Eq14'.
-                                     injection Eq12  as Eq12.  rewrite Eq12.
-                                     rewrite word_add_x_0_is_x. reflexivity.
-                                 +++ assert (Eq14' := stack_val_has_value_eval c arg3 WZero m1' ops Eq14).
-                                     rewrite Eq13 in Eq14'. 
-                                     injection Eq14' as Eq14'. rewrite Eq14'.
-                                     destruct m1' eqn:Eq17.
-                                     ++++ simpl in Eq12.                                      
-                                          rewrite word_add_x_0_is_x. simpl.
-                                          rewrite Eq12. reflexivity.
-                                     ++++ exfalso. apply (th6 p0 l). assumption.
-                                 +++ assert (Eq14' := stack_val_has_value_eval c arg3 WZero m1' ops Eq14).
-                                     rewrite Eq13 in Eq14'. 
-                                     injection Eq14' as Eq14'. rewrite Eq14'.
-                                     rewrite word_add_x_0_is_x.
-                                     assert (Eq15' := th7 m1' Eq15). rewrite Eq15' in Eq12.
-                                     rewrite Eq12. reflexivity.
-                              ++ pose proof (IH (p0::a) ops c H1 Eq15) as HH.
-                                 rewrite <- HH. rewrite Eq12.
-                                 assert (Eq14' := stack_val_has_value_eval c arg3 WZero m1' ops Eq14).
-                                 rewrite Eq13 in Eq14'. 
-                                 injection Eq14' as Eq14'. rewrite Eq14'.
-                                 rewrite word_add_x_0_is_x. reflexivity.
-                            + rewrite H1. rewrite -> eval_asfs2_ho.
-                              destruct (opt_map' opt_add_0_elem m1') eqn:Eq15.
-                              ++ 
-                                 destruct arg2 eqn:Eq16.
-                                 destruct arg3 eqn:Eq17.
-                                 +++ rewrite eval_value in Eq12. injection Eq12 as Eq12.
-                                     rewrite eval_value in Eq13. injection Eq13 as Eq13.
-                                     rewrite Eq12. rewrite Eq13.
-                                     reflexivity.
-                                 +++ rewrite eval_value in Eq12. injection Eq12 as Eq12.
-                                     destruct (nth_error c var) eqn:Eq18.
-                                     ++++ rewrite (th8 c var m1' ops) in Eq13.
-                                          cbn. rewrite Eq12. rewrite Eq18.
-                                          rewrite Eq13 in Eq18. injection Eq18 as Eq18.
-                                          rewrite Eq18. reflexivity.
-                                     ++++ rewrite (th8 c var m1' ops) in Eq13.
-                                          rewrite Eq13 in Eq18. discriminate.
-
-                                 +++ rewrite eval_value in Eq12. injection Eq12 as E12.
-                                     assert (Eq15':= th7 m1' Eq15).
-                                     rewrite Eq15' in Eq13.
-                                     simpl in Eq13. discriminate.
-                                 +++ assert (Eq15':= th7 m1' Eq15).
-                                     rewrite Eq15' in Eq12.
-                                     simpl in Eq12.
-                                     cbn. rewrite Eq12.
-                                     destruct arg3 eqn:Eq18.
-                                     ++++ rewrite eval_value in Eq13. injection Eq13 as Eq13.
-                                          rewrite Eq13. reflexivity.
-                                     ++++ rewrite (th8 c var0 m1' ops) in Eq13.
-                                          rewrite Eq13. reflexivity.
-                                     ++++ rewrite Eq15' in Eq13. simpl in Eq13. discriminate. 
-                                 +++ assert (Eq15':= th7 m1' Eq15).
-                                     rewrite Eq15' in Eq12. simpl in Eq12. discriminate. 
-
-
-
-                              ++ pose proof (IH (p0::a) ops c H1 Eq15) as HH.
-                                 destruct arg2 eqn:Eq16.
-                                 destruct arg3 eqn:Eq17.
-                                 +++ rewrite eval_value in Eq12. injection Eq12 as Eq12.
-                                     rewrite eval_value in Eq13. injection Eq13 as Eq13.
-                                     rewrite Eq12. rewrite Eq13.
-                                     reflexivity.
-                                 +++ rewrite eval_value in Eq12. injection Eq12 as Eq12.
-                                     destruct (nth_error c var) eqn:Eq18.
-                                     ++++ rewrite (th8 c var m1' ops) in Eq13.
-                                          cbn. rewrite Eq12. rewrite Eq18.
-                                          rewrite Eq13 in Eq18. injection Eq18 as Eq18.
-                                          rewrite Eq18. reflexivity.
-                                     ++++ rewrite (th8 c var m1' ops) in Eq13.
-                                          rewrite Eq13 in Eq18. discriminate.
-                                 +++ rewrite eval_value in Eq12. injection Eq12 as E12.
-                                     destruct m1' eqn:Eq18.
-                                     ++++ cbn in Eq13. discriminate.
-                                     ++++ simpl. admit.
-                                 +++ admit.
-                                 +++ destruct m1' eqn:E18.
-                                     ++++ simpl in Eq12. discriminate.
-                                     ++++ simpl. admit. 
-            
-                      ----- admit.
-                 ---- admit.
- 
-          -- destruct (ops MUL) eqn:Eq5; try reflexivity.
-             destruct o eqn:Eq6.
-             destruct (length args =? nb_args) eqn:Eq7; try reflexivity.
-             destruct (opt_map' opt_add_0_elem m1') eqn:Eq8.
-             --- assert (Eq8' := th7 m1' Eq8). rewrite Eq8'. reflexivity.
-             --- pose proof (IH (p::a) ops c H1 Eq8) as HH.
-                 rewrite -> eval_asfs2_ho. rewrite -> eval_asfs2_ho.
-                 assert (HH2 := eq_eval_elem_stack c m1' (p::a) ops args HH).
-                 rewrite <- HH2. reflexivity.
-          -- destruct (ops NOT) eqn:Eq5; try reflexivity.
-             destruct o eqn:Eq6.
-             destruct (length args =? nb_args) eqn:Eq7; try reflexivity.
-             destruct (opt_map' opt_add_0_elem m1') eqn:Eq8.
-             --- assert (Eq8' := th7 m1' Eq8). rewrite Eq8'. reflexivity.
-             --- pose proof (IH (p::a) ops c H1 Eq8) as HH.
-                 rewrite -> eval_asfs2_ho. rewrite -> eval_asfs2_ho.
-                 assert (HH2 := eq_eval_elem_stack c m1' (p::a) ops args HH).
-                 rewrite <- HH2. reflexivity.
+                        ++ rewrite <- H2. simpl. rewrite Eq9. reflexivity.
+                ----- destruct (stack_val_has_value arg2 WZero) eqn:Eq8.
+                      + assert (Eq8' := stack_val_has_value_eval c arg2 WZero m1' ops Eq8).
+                        destruct e as [val|var|fvar] eqn:Eq9.
+                        ++ rewrite <- H2. apply eval_value.
+                        ++ rewrite <- H2. apply eval_var.
+                        ++ simpl. destruct (id =? fvar) eqn:Eq10.
+                           +++ rewrite H1. rewrite Eq8'.
+                               destruct (eval_asfs2_elem c arg1 m1' ops) eqn:Eq11;
+                                try rewrite word_add_x_0_is_x;
+                                try (
+                                    rewrite <- H2; simpl; rewrite Eq10; 
+                                    rewrite Eq11; reflexivity).
+                           +++ rewrite <- H2. simpl. rewrite Eq10. reflexivity.
+                      + destruct e as [val|var|fvar] eqn:Eq9.
+                        ++ rewrite <- H2. reflexivity.
+                        ++ rewrite <- H2. reflexivity.
+                        ++ simpl. destruct (id =? fvar) eqn:Eq10.
+                           +++ rewrite H1.
+                               destruct (eval_asfs2_elem c arg1 m1' ops) eqn:Eq11.
+                               ++++ destruct (eval_asfs2_elem c arg2 m1' ops) eqn:Eq12.
+                                    +++++ rewrite <- H2. simpl.
+                                          rewrite Eq10. rewrite H1.
+                                          rewrite Eq11. rewrite Eq12.
+                                          reflexivity.
+                                    +++++ rewrite <- H2. simpl.
+                                          rewrite Eq10. rewrite H1.
+                                          rewrite Eq11. rewrite Eq12.
+                                          reflexivity.
+                               ++++ rewrite <- H2. simpl.
+                                    rewrite Eq10. rewrite H1.
+                                    rewrite Eq11. reflexivity.
+                           +++ rewrite <- H2. simpl. rewrite Eq10. reflexivity.
+           ---- rewrite <- H2. rewrite Eq1'. reflexivity.
+           ---- rewrite <- H2. rewrite Eq1'. reflexivity.
+    -- destruct e as [val|var|fvar] eqn:Eq2.
+       --- rewrite <- H2. rewrite eval_value. rewrite eval_value. reflexivity.
+       --- rewrite <- H2. apply eval_var.
+       --- rewrite <- H2. simpl. destruct (id' =? fvar) eqn:Eq3.
+           ---- destruct v as [bv|opval] eqn:Eq4.
+                ----- destruct bv as [val'|var'|fvar'] eqn:Eq5.
+                      + admit.
+                      + admit.
+                      + admit.
+                ----- destruct (ops opval) eqn:Eq5.
+                      destruct o eqn:Eq6.
+                      destruct (length args =? nb_args) eqn:Eq7.
+                      + rewrite -> eval_asfs2_ho.
+                        destruct m1'.
+                        ++ admit.
+                        ++ admit.
+                      + admit.
+                      + admit.
+           ---- apply IH with (id:=id); try assumption; try reflexivity.
 
 Admitted.
+
+
 
 Theorem th_opt_add_0_correct: forall (c1 c2: concrete_stack) (a1 a2 : asfs) (ops: opm),
   length c1 = get_height_asfs a1 ->
